Subst.v
@@ -11,6 +11,13 @@ Definition subst_t (X : Type) := list (X * X).
 Class Subst (A X : Type) : Type :=
   subst: subst_t X -> A -> A.
 
+Fixpoint subst_prod (A X : Type) (SX : Subst X X) (s : subst_t X) (p : (X * A)) :=
+  match p with
+    | (p1, p2) => (subst s p1, p2)
+  end.
+
+Instance Subst_prod (A X : Type) (SX : Subst X X) : Subst (X * A) X := subst_prod A X SX.
+
 Fixpoint subst_list (A X : Type) (SAX : Subst A X) (s : subst_t X) (l : list A) :=
   match l with
     | nil => nil
@@ -18,3 +25,9 @@ Fixpoint subst_list (A X : Type) (SAX : Subst A X) (s : subst_t X) (l : list A) 
   end.
   
 Instance Subst_list (A X : Type) (SAX : Subst A X) : Subst (list A) X := subst_list A X SAX.
+
+Instance Subst_prod_list (A X : Type) (S : Subst X X) : Subst (list (X * A)) X := 
+  subst_list (X * A) X (Subst_prod A X S).
+
+Definition wf_subst (X : Type) (s : subst_t X) :=
+  NoDup (fst (split s)).
