Translation.v
@@ -1,4 +1,5 @@
 Add LoadPath "vst".
+Require Import CpdtTactics.
 Require Import Types.
 Require Import ProgramLogic.
 Require Import Language.
@@ -8,13 +9,46 @@ Require Import List.
 Require Import msl.msl_direct.
 Require Import Coq.Unicode.Utf8.
 
+Set Implicit Arguments.
+
+(* Require String. Open Scope string_scope. *)
+
+(* Ltac move_to_top x := *)
+(*   match reverse goal with *)
+(*   | H : _ |- _ => try move x after H *)
+(*   end. *)
+
+(* Tactic Notation "assert_eq" ident(x) constr(v) := *)
+(*   let H := fresh in *)
+(*   assert (x = v) as H by reflexivity; *)
+(*   clear H. *)
+
+(* Tactic Notation "Case_aux" ident(x) constr(name) := *)
+(*   first [ *)
+(*     set (x := name); move_to_top x *)
+(*   | assert_eq x name; move_to_top x *)
+(*   | fail 1 "because we are working on a different case" ]. *)
+
+(* Tactic Notation "Case" constr(name) := Case_aux Case name. *)
+(* Tactic Notation "SCase" constr(name) := Case_aux SCase name. *)
+(* Tactic Notation "SSCase" constr(name) := Case_aux SSCase name. *)
+(* Tactic Notation "SSSCase" constr(name) := Case_aux SSSCase name. *)
+(* Tactic Notation "SSSSCase" constr(name) := Case_aux SSSSCase name. *)
+(* Tactic Notation "SSSSSCase" constr(name) := Case_aux SSSSSCase name. *)
+(* Tactic Notation "SSSSSSCase" constr(name) := Case_aux SSSSSSCase name. *)
+(* Tactic Notation "SSSSSSSCase" constr(name) := Case_aux SSSSSSSCase name. *)
+
 Open Scope pred.
 
+(** Preliminaries ??? **)
+Definition subst_pred (x: var) (e: expr) (p: pred world) : pred world :=
+  fun w =>
+    let w' := fun x' => if eq_dec x x' then eval w e else w x' in
+    p w'.
+
+(** The meat of the sauce :d tasty **)
 Definition sep_base (x:var) (t:base_type) : pred world :=
-  match t with
-    | int_t => EX v : nat, (fun s => (eval s (var_e x) = Some (int_v v)))
-    | bool_t => EX v : bool, (fun s => (eval s (var_e x) = Some (bool_v v)))
-  end.
+  EX v : (base_of_type t), (fun s => (eval s (var_e x) = Some (val_of_base t v))).
 
 Fixpoint sep_pred (p:reft_prop) : pred world :=
   match p with
@@ -32,14 +66,15 @@ Fixpoint sep_pred (p:reft_prop) : pred world :=
           && (fun s => Some (int_v v1) = (eval s e1)) 
           && (fun s => Some (int_v v2) = (eval s e2))
       end
-    | not_r p => imp (sep_pred p) FF
+    | not_r p => (sep_pred p) --> FF
     | and_r p1 p2 => sep_pred p1 && sep_pred p2
     | or_r p1 p2 => sep_pred p1 || sep_pred p2
   end.
 
 Definition sep_ty (x:var) (t:reft_type) : pred world :=
   match t with
-  | mkReft_type v b p => sep_base x b && sep_pred (subst ((v,x) :: nil) p)
+  | mkReft_type v b p => sep_base x b 
+                      && (sep_pred (subst ((v,x) :: nil) p))
   end.
 
 Fixpoint sep_env (Γ : type_env) : pred world :=
@@ -47,40 +82,4 @@ Fixpoint sep_env (Γ : type_env) : pred world :=
     | nil => TT
     | (x,t) :: Γ' => sep_ty x t && sep_env Γ'
   end.
-
-Lemma var_eval :
-  forall Γ x t,  (x,t) ∈ Γ -> (sep_env Γ |-- (fun s => eval s (var_e x) <> None)).
-Proof.
-  intros Γ.
-  induction Γ as [ | xt].
-  intros x t X w H v. auto.
-  intros x t X w H v.
-  specialize IHΓ with (x := x) (t := t).
-  destruct t as [ vv b p ].
-  apply in_inv in X.
-  destruct X.
-  (* assert (w x <> None). *)
-  unfold sep_env in H. simpl in *. unfold sep_ty in H. unfold sep_pred in H.
-  subst.
-  destruct H as [[A B] C]. 
-  clear B C.
-  unfold sep_base in A. destruct b. 
-   simpl in *.
-     unfold exp in A. 
-     rewrite v in A. elim A. intros. inversion H. 
-   simpl in *.
-    unfold exp in A.
-    rewrite v in A. elim A. intros. inversion H.
-  assert (eval w x <> None).
-  apply IHΓ.
-  apply H0.
-  unfold sep_env in H. destruct xt. destruct H as [A B].
-  fold sep_env in B. apply B. rewrite v in H1. auto.
-Qed.
-
-(* Lemma expr_eval :
-  forall Γ e t,
-    expr_type Γ e t -> (sep_env Γ) |-- (EX v : value, (fun s => eval s e = Some v)).
-Proof.
-  Admitted.
-Qed. *)
+  
