EvalLemmas.v
@@ -1,0 +1,69 @@
+Add LoadPath "vst".
+Require Import msl.msl_direct.
+Require Import Coq.Unicode.Utf8.
+
+Require Import Translation.
+Require Import WFLemmas.
+Require Import SubstLemmas.
+Require Import Types.
+Require Import Judge.
+Require Import Language.
+Require Import Tactics.
+
+Lemma var_val : 
+  forall Γ x ν b φ w,  (x,{ ν : b | φ}) ∈ Γ -> 
+                       sep_env Γ w -> 
+                       (EX v : (base_of_type b), 
+                               (fun s => eval s (var_e x) = Some (val_of_base b v))) w.
+Proof.
+  induction Γ; repeat crush_sep False fail.  
+Qed.
+
+Lemma var_eval :
+  forall Γ x t w, (x,t) ∈ Γ -> sep_env Γ w -> (EX v : value, (fun s => eval s (var_e x) = Some v)) w.
+Proof.
+  destruct t as [ν b φ]; crush_sep var_val fail.
+Qed.
+
+Lemma expr_eval : 
+  forall Γ e T w, 
+    sep_env Γ w -> expr_type Γ e T ->
+                (EX v : value, (fun s => eval s e = Some v)) w.
+Proof.
+  autounfold in *. intros. crush_sep False fail. 
+  destruct e as [v | x]. 
+    crush_sep False fail.
+    inversion H0; apply var_eval with (Γ := Γ) (t:= T);
+    crush.
+Qed.
+
+Lemma expr_eval_ty :
+  forall Γ e b φ w, 
+    sep_env Γ w -> expr_type Γ e { ν : b | φ } -> 
+      (EX v : base_of_type b , (fun s => eval s e = Some (val_of_base b v))) w.
+Proof.
+  autounfold in *. intros.
+  destruct e. 
+  + destruct b.
+  - inversion H0. subst.
+    destruct v. 
+    * simpl. exists n. reflexivity.
+    * simpl. exists b. reflexivity.
+  - inversion H0. subst.
+    destruct v.
+    * simpl. exists n. reflexivity.
+    * simpl. exists b. reflexivity.
+  + inversion H0. subst.
+    * simpl. pose (var_val Γ v ν b φ w H4 H). assumption.
+Qed.
+
+Lemma expr_eval_derives :
+  forall Γ e t,
+    expr_type Γ e t -> (sep_env Γ) |-- (EX v : value, (fun s => eval s e = Some v)).
+Proof.
+  intros Γ e t T w Den_Γ.
+  destruct e.
+  exists v. reflexivity.
+  apply var_eval with (x := v) (t:=t) in Den_Γ .
+  auto. inversion T. apply H1.
+Qed.
