Logic.v
@@ -1,0 +1,168 @@
+Add LoadPath "vst".
+Require Import msl.msl_direct.
+Require Export Lang.
+
+Delimit Scope logic_scope with logic.
+
+Definition world := var -> option value.
+Definition den (s: state) : world := table_get s.
+Definition defined (y: var) : pred world :=
+   fun w => exists v, w y = Some v.
+
+Definition eval_to (e: expr) (v:value) : pred world :=
+  fun w => eval w e = Some v.
+
+Instance Join_world: Join world := Join_equiv world.
+
+Instance Perm_world : Perm_alg world := _.
+Instance Sep_world : Sep_alg world := _.
+Instance Canc_world : Canc_alg world := _.
+Instance Disj_world : Disj_alg world := _.
+
+Definition fun_set (f: var -> option value) (x: var) (y: option value) :=
+  fun i => if eq_dec i x then y else f i.
+
+Definition subst (x : var) (v : option value) (P: pred world) : (pred world) := 
+  fun w => P (fun_set w x v).
+
+Definition equal (x y: var) : pred world :=
+  fun w => w x = w y.
+
+Inductive modvars : stmt -> var -> Prop :=
+| mod_assign: forall x e, modvars (assign_s x e) x
+| mod_seq1: forall x s1 s2, modvars s1 x -> modvars (seq_s s1 s2) x
+| mod_seq2: forall x s1 s2, modvars s2 x -> modvars (seq_s s1 s2) x.
+
+Definition nonfreevars (P: pred world) (x: var) : Prop :=
+  forall stk v, P stk -> P (fun_set stk x v).
+
+Definition subset (S1 S2 : var -> Prop) := forall x, S1 x -> S2 x.
+
+Inductive safe : (list stmt * state) -> Prop :=
+| safe_step: forall s1 s2, step s1 s2 -> safe s2 -> safe s1
+| safe_halt: forall s, safe (nil, s).
+
+Definition guards (P: pred world) (ss : list stmt) : Prop :=
+  forall s, P (den s) -> safe (ss, s).
+
+Definition semax (P: pred world) (s: stmt) (Q: pred world): Prop :=
+  forall F, subset (modvars s) (nonfreevars F) ->
+    forall k, guards (Q * F) k -> guards (P * F) (s :: k).
+
+Notation "{{ P }} s {{ Q }}" := (semax P%pred s Q%pred) (at level 90).
+
+Lemma semax_skip:
+  forall P, {{ P }} skip_s {{ P }}. (*(semax P skip_s P).*)
+Proof.
+  intros P.
+  unfold semax.
+  intros F H k HG st HP.
+  eapply safe_step. constructor. 
+  eauto.
+Qed.
+
+Lemma semax_seq:
+  forall P Q R s1 s2, 
+    {{ P }} s1 {{ Q }} -> {{ Q }} s2 {{ R }} -> 
+    {{ P }} seq_s s1 s2 {{ R }} .
+Proof.  
+  intros P Q R s1 s2.
+  intros S1 S2.
+  intros F H k H0 s H1.
+  assert (safe ( s1 :: s2 :: k, s)).
+  Focus 2.
+    inv H2; eapply safe_step; [constructor | eauto]; auto.
+  apply (S1 F); auto.
+  intros ? ?. apply H. apply mod_seq1. auto.
+  apply S2.
+  intros ? ?. apply H. apply mod_seq2. auto.
+  auto.
+Qed.
+
+Lemma semax_assign:
+  forall P x e v,
+    {{ (subst x (Some v) P && eval_to e v) }} assign_s x e {{ P }}.
+Proof.
+  intros P x e v.
+  intros F S k H0 st H1.
+  destruct H1 as [stk1 [stk2 [A [[B C] D]]]].
+  destruct A as [E1 E2]. rewrite E2 in *. 
+  eapply safe_step. constructor.
+  unfold eval_to in C.
+  unfold den in *.
+  rewrite <- E1. symmetry in C. apply C.
+  apply H0.
+  exists (fun_set (table_get st) x (Some v)). 
+  exists (fun_set (table_get st) x (Some v)). 
+  split; [| split].
+  split; auto.
+  unfold den in *.
+  unfold subst in B. rewrite <- E1. apply B.
+  unfold den in *. 
+  apply (S x).
+  apply mod_assign. 
+  assumption.
+Qed.
+
+Lemma semax_frame:
+  forall F P s Q,
+    subset (modvars s) (nonfreevars F) ->
+    {{ P }} s {{ Q }} ->
+    {{ (P * F) }} s {{ (Q * F) }}.
+Proof.
+  repeat intro.
+  rewrite sepcon_assoc in H2,H3. 
+  assert (guards (P * (F * F0)) (s :: k)).
+  apply H0. intros ? ?. 
+  unfold subset in H.
+  specialize (H x H4).
+  specialize (H1 _ H4).
+  repeat intro. 
+  destruct H5 as [stk1 [stk2 [[? ?] [? ?]]]].
+  subst.
+  exists (fun_set stk x v).
+  exists (fun_set stk x v).
+  split; auto.
+  split; auto. 
+  apply H2; auto.
+  apply H4; auto.
+Qed.
+
+Lemma semax_consequence:
+  forall P P' s Q Q',
+   P |-- P' -> Q' |-- Q -> {{ P' }} s {{ Q' }} ->
+   {{ P }} s {{ Q }}.
+Proof.
+  repeat intro.
+  apply (H1 F); auto.
+  intros ? ?.
+  apply H3.
+  eapply sepcon_derives; try apply H5; auto.
+  eapply sepcon_derives; try apply H4; auto.
+Qed.
+
+ 
+Example ex1: 
+  {{ fun s => s 0 = (Some (int_v 0)) }} skip_s {{ TT }}.
+Proof.
+  eapply semax_consequence with (P' := TT) (Q' := TT) .
+  repeat intro. constructor. constructor.
+  apply semax_skip.
+Qed.
+
+Definition x : var := 0.
+Definition one := int_v 1.
+Definition n : expr := (value_e one).
+Definition P := fun s => eval s x = Some one.
+
+Example ex2:
+  {{ TT }} assign_s x n {{ P }}.
+Proof.
+  apply semax_consequence with 
+    (P' := (subst x (Some one) P && eval_to n one)%pred) (Q' := P).
+  repeat intro. unfold P. unfold subst. unfold fun_set. 
+  split; reflexivity. auto.
+  apply semax_assign.
+Qed.
+
+(* ; specialize (H1 _ H4). *)
