SubstLemmas.v
@@ -1,0 +1,228 @@
+Add LoadPath "vst".
+Require Import msl.msl_direct.
+Require Import Coq.Unicode.Utf8.
+
+Require Import Translation.
+Require Import Types.
+Require Import Judge.
+Require Import Language.
+Require Import Subst.
+Require Import WFLemmas.
+Require Import Tactics.
+
+Lemma subst_none_base :
+  forall x e x' t' s,
+   x <> x' -> (subst_pred x e (sep_base x' t') s) -> (sep_base x' t' s).
+Proof.
+  autounfold in *; crush_sep False fail; destruct (eq_dec x x') eqn:EQ; crush.
+Qed.
+
+Lemma subst_none_base' :
+  forall x e x' t' s,
+   x <> x' -> (sep_base x' t' s) -> (subst_pred x e (sep_base x' t') s).
+Proof.
+  autounfold in *; crush_sep False fail; destruct (eq_dec x x') eqn:EQ; crush.
+Qed.
+
+Lemma not_prop_1 :
+  forall φ w,
+    sep_pred (not_r φ) w -> (sep_pred φ) w -> FF w.
+Proof.
+  crush.
+Qed.
+
+Lemma not_prop_2 :
+  forall φ w,
+    sep_pred φ w -> FF w -> sep_pred (not_r φ) w.
+Proof.
+  crush.
+Qed.
+  
+Lemma subst_not :
+  forall x e φ w,
+    subst_pred x e (sep_pred (not_r φ)) w -> (subst_pred x e (sep_pred φ) w -> FF w).
+Proof.
+  crush.
+Qed.
+
+Lemma not_inv:
+  forall p q w,
+    sep_pred p w -> sep_pred q w -> sep_pred (not_r q) w -> sep_pred (not_r p) w.
+Proof.
+  crush.
+Qed.
+
+Lemma not_inv2:
+  forall p q w,
+    sep_pred p w -> sep_pred (not_r q) w -> sep_pred q w -> sep_pred (not_r p) w.
+Proof.
+  crush.
+Qed.
+
+Lemma subst_none_eq :
+  forall x e Γ ν τ e1 e2 s,
+    var_not_in x Γ -> wf_type Γ { ν : τ | e1 .= e2 } -> (x <> ν) -> 
+    (subst_pred x e (sep_pred (e1 .= e2)) s <-> sep_pred (e1 .= e2) s).
+    (* /\ (sep_pred (e1 .= e2) s -> subst_pred x e (sep_pred (e1 .= e2)) s)). *)
+Proof.
+  unfold subst_pred;
+  crush' var_not_in_exp (wf_expr, wf_prop, wf_type);
+  destruct e1 eqn:E1; 
+  destruct e2 eqn:E2;
+  crush_sep False fail;
+    repeat match goal with
+             | [ H: context[eq_dec ?x ?y] |- _ ] => destruct (eq_dec x y)
+             | |- context[eq_dec ?x ?y] => destruct (eq_dec x y)
+             | |- appcontext[( _ && _ )] => split; simpl
+          end; crush.
+Qed.
+
+Lemma subst_none_lt :
+ forall x e Γ ν τ e1 e2 s,
+    var_not_in x Γ -> wf_type Γ { ν : τ | e1 .< e2 } -> x <> ν ->
+    (subst_pred x e (sep_pred (e1 .< e2)) s <-> sep_pred (e1 .< e2) s).
+Proof.
+  unfold subst_pred;
+  crush' var_not_in_exp (wf_expr, wf_prop, wf_type);
+  destruct e1;
+  destruct e2;
+  reduce_preds;
+    repeat (match goal with
+              | [ x:_, y:_, H:appcontext[!!(?x < ?y)] |- _] => exists x; exists y; simpl
+              | [ H: context[eq_dec ?x ?y] |- _ ] => destruct (eq_dec x y)
+              | |- context[eq_dec ?x ?y] => destruct (eq_dec x y)
+              | |- appcontext[( _ && _ )] => split; simpl
+            end; crush).
+Qed.
+
+Lemma subst_none_rel :
+ forall x e Γ ν τ b e1 e2 s,
+    var_not_in x Γ -> wf_type Γ { ν : τ | rel_r e1 b e2 } -> x <> ν ->
+    (subst_pred x e (sep_pred (rel_r e1 b e2)) s <-> sep_pred (rel_r e1 b e2) s).
+Proof.
+  destruct b. apply subst_none_eq. apply subst_none_lt.
+Qed.
+
+Lemma subst_not_1 :
+  forall φ s,
+    (sep_pred (not_r φ) s -> (sep_pred φ s -> FF s)).
+Proof.
+  crush.
+Qed.
+
+Lemma subst_not_2 :
+  forall φ s,
+    (sep_pred φ s -> FF s) -> (sep_pred (not_r φ) s).
+Proof.
+  crush.
+Qed.
+
+Lemma subst_none_prop :
+  forall φ x e Γ τ s,
+    var_not_in x Γ -> wf_type Γ { ν : τ | φ } -> x <> ν ->
+    (subst_pred x e (sep_pred φ) s <-> sep_pred φ s).
+Proof.
+  Ltac autocons := 
+    repeat (econstructor || app_pred || eauto); crush.
+  Ltac t :=
+    first [btapply autocons | solve [left; btapply autocons] | solve [right; btapply autocons]].
+  intro φ.
+  induction φ.
+  (* true *)
+  crush. 
+  (* rel *)
+  intros; apply subst_none_rel with (Γ := Γ) (ν := ν) (τ := τ); auto.
+  (* not *)
+  wf_crush; t.
+  (* and  *)
+  wf_crush; t.
+  (* or *)
+  wf_crush; t. 
+Qed.
+
+Lemma subst_commute :
+  forall (x y : var) (x' y' : expr) p s,
+    (var_e y) <> x' -> (var_e x) <> y' -> x <> y -> x' <> y' ->
+    subst_pred x x' (subst_pred y y' p) s =
+      subst_pred y y' (subst_pred x x' p) s.
+Proof.
+  intros. unfold subst_pred. f_equal.
+  destruct x' as [x'v | x']. 
+    extensionality. simpl.
+      destruct y' as [y'v | y'].
+        destruct (eq_dec x x0). 
+          destruct (eq_dec y x0). 
+            rewrite e in H1. rewrite e0 in H1. exfalso. apply H1; reflexivity.
+            reflexivity.
+          destruct (eq_dec y x0).
+            rewrite e in H1. reflexivity.
+            reflexivity.
+        destruct (eq_dec x x0).
+          destruct (eq_dec y x0). 
+            rewrite e in H1. rewrite e0 in H1. exfalso. apply H1; reflexivity.
+            reflexivity.
+          destruct (eq_dec y x0). 
+            simpl. destruct (eq_dec x y'). 
+              rewrite e0 in H0. contradiction H0. reflexivity.
+              reflexivity.
+            reflexivity.
+    extensionality. simpl.
+      destruct y' as [y'v | y'].
+        destruct (eq_dec y x0).
+          simpl. destruct (eq_dec x x0).
+            rewrite e in H1. rewrite e0 in H1. contradiction H1. reflexivity.
+            reflexivity. 
+        destruct (eq_dec x x0). simpl.
+          destruct (eq_dec y x'). 
+            rewrite e0 in H. contradiction H. reflexivity.
+            reflexivity.
+          reflexivity.
+       destruct (eq_dec y x0). simpl.
+         destruct (eq_dec x y'). rewrite e0 in H0. contradiction H0. reflexivity.
+         destruct (eq_dec y x'). rewrite e0 in H. contradiction H. reflexivity. 
+         destruct (eq_dec x x0). rewrite e in H1. rewrite e0 in H1. contradiction H1. reflexivity.
+         reflexivity.
+         destruct (eq_dec y x'). rewrite e in H. contradiction H. reflexivity.
+         reflexivity.
+Qed.
+
+Lemma subst_none_ty : 
+  forall Γ x x' e T s, 
+    x <> ν -> x' <> ν -> var_e ν <> e -> x <> x' ->
+    var_not_in x Γ -> wf_type Γ T -> var_in x' Γ ->
+    (subst_pred x e (sep_ty x' T) s -> sep_ty x' T s).
+Proof.
+  intros Γ x x' e T s neq_x_vv neq_x'_vv neq_e_vv neq_x_x' NotIn WF_Type VarIn.
+  inversion WF_Type; subst.
+  intro SubSep; destruct SubSep as [SepBase SepTy]; apply subst_none_base in SepBase.
+  unfold sep_ty. split. assumption.
+  fold (subst_pred x e (sep_pred (subst ((ν,x')::nil) p)) s) in SepTy.
+  pose subst_none_prop as Foo.
+  specialize (Foo (subst ((ν,x') :: nil) p) x e Γ b s NotIn).
+  apply Foo.
+  apply wf_reft_t. apply wf_prop_subst. 
+  assumption.
+  assumption.
+  assumption.
+  assumption.
+  assumption.
+Qed.
+
+Lemma subst_none_ty' :
+  forall Γ x x' e T s, 
+    x <> ν -> x' <> ν -> var_e ν <> e -> x <> x' ->
+    var_not_in x Γ -> wf_type Γ T -> var_in x' Γ ->
+    (sep_ty x' T s -> subst_pred x e (sep_ty x' T) s ).
+Proof.
+  intros Γ x x' e T s neq_x_vv neq_x'_vv neq_e_vv neq_x_x' NotIn WF_Type VarIn.
+  inversion WF_Type; subst.
+  intro SepTy. destruct SepTy as [SepBase SepPred].
+  apply subst_none_base' with (x := x) (e := e) (x' := x') (t' := b) in SepBase.
+  2: assumption.
+  unfold sep_ty.
+  split. assumption.
+  pose subst_none_prop as foo.
+  specialize (foo (subst ((ν,x')::nil) p) x e Γ b s NotIn). 
+  apply foo.
+  apply wf_reft_t. apply wf_prop_subst. assumption. assumption. assumption. assumption.
+Qed.
