Tactics.v
@@ -1,0 +1,221 @@
+Add LoadPath "vst".
+Require Export CpdtTactics.
+Require Import Types.
+Require Import Judge.
+Require Import Subst.
+Require Import ProgramLogic.
+Require Import Language.
+Require Import Translation.
+Require Import msl.msl_direct.
+Require Import Coq.Unicode.Utf8.
+
+(** Generally Useful ?? **)
+Hint Unfold var_not_in.
+Hint Unfold var_in.
+Hint Unfold wf_env.
+Hint Unfold Subst_var_expr.
+Hint Unfold subst.
+Hint Unfold derives.
+Hint Unfold imp.
+Hint Unfold subst_pred.
+Hint Unfold sep_base.
+
+Hint Rewrite -> Forall_forall.
+Hint Rewrite -> in_inv.
+
+Hint Resolve in_inv.
+
+Hint Constructors wf_prop.
+
+Open Scope pred.
+
+Ltac eval_refl :=
+  match goal with
+    | [Q : Some _ = eval _ (_ ?e1),
+       R : Some _ = eval _ (_ ?e2)
+       |- @eq (option value) (Some ?e1) (_ _ (_ ?e2)) ] =>
+      simpl in *; try eval_refl
+
+    | [ P : Some ?v = _, 
+        Q : Some ?v = _ 
+        |- Some ?v = eval _ _ ] => simpl in *; try eval_refl
+
+
+    | P : ?T |- ?T => assumption
+
+    | [ H: ?x <> ?y,
+        P: Some _ = (if eq_dec ?x ?y then _ else _)
+      |- Some _ = eval _ _ ] =>
+      let e0 := fresh "e0" in
+      destruct (eq_dec x y) as [ e0 | e0 ];
+      [ rewrite e0 in H; contradiction H; auto | auto ]
+                                                 
+    | [ V: (var_e ?x' <> var_e ?x),
+        H: Some ?v = (if eq_dec ?x ?x' then _ else ?v')
+        |- Some ?v = ?v' ] =>
+        let e0 := fresh "e0" in
+        destruct (eq_dec x x') as [ e0 | e0];
+        [ rewrite e0 in V; contradiction V; auto | auto ]
+
+     |[ V : var_e ?x' <> var_e ?x,
+        P : Some ?v = ?eval
+        |- Some ?v = (if eq_dec ?x ?x' then _ else ?eval)] =>
+        let e0 := fresh "e0" in
+        destruct (eq_dec x x') as [ e0 | e0 ];
+        [ rewrite e0 in V; contradiction V; auto | auto ]
+
+    | [ V : (var_e ?e2 <> var_e ?x),
+        Q : Some ?v = _,
+        R : Some ?v = (if eq_dec ?x ?e2 then _ else _)
+        |- @eq (option value) (Some ?e1) (_ ?e2) ] =>
+        let e0 := fresh "e0" in
+        try (rewrite <- Q; rewrite R); destruct (eq_dec x e2) as [ e0 | e0 ];
+        [ rewrite e0 in V; contradiction V; auto | auto ]; try assumption
+
+     |[ V : var_e ?ex2 ≠ var_e ?x,
+        P : Some ?v = _,
+        Q : Some ?v = _ ?ex2
+        |- Some _ = (if eq_dec ?x ?ex2 then _ else _ ?ex2)] =>
+        let e0 := fresh "e0" in
+        try (rewrite <- P; rewrite Q); destruct (eq_dec x ex2) as [ e0 | e0 ];
+        [ rewrite e0 in V; contradiction V; auto | auto ]
+
+    | [ e1:value, e2:value,
+       Q : Some _ = Some ?e1,
+       R : Some _ = Some ?e2
+        |- (Some ?e1) = (Some ?e2) ] =>
+      rewrite <- Q; rewrite R; reflexivity
+
+    | [Q : Some ?e1 = eval _ _,
+       R : Some ?e1 = eval _ _
+       |- (Some ?e1) = _ ] =>
+      simpl in *; try eval_refl
+
+    | [ P : ?e <> (var_e ?x),
+        Q : Some ?v = eval _ ?e
+        |- Some ?v = eval _ ?e ] => destruct e; simpl in *; try (assumption ||  eval_refl)
+  end.
+
+Ltac crush_eval := 
+  match goal with
+    |         |- Some _ = eval _ _ => eval_refl
+    | e2:expr |- Some _ = _ _ ?e2 => destruct e2; eval_refl
+  end.
+
+Ltac freshvar :=
+  match goal with
+    | [ Γ:_, x:_, H1 :_, I : In ?p _ |- _] => 
+      let H := fresh "H" in
+      set (H := H1);
+      unfold var_not_in in H; 
+      rewrite Forall_forall in H;
+      specialize (H p I);
+      simpl in H
+  end.
+
+Ltac app_pair :=
+  match goal with 
+    | [ x : _, t : _, H : _ |- _ ] => specialize (H (x, t))
+  end.
+
+Ltac pair_crush' lems invs := 
+  crush' lems invs 
+  || app_pair; try crush' lems invs 
+  || crush' lems invs ; app_pair; try crush' lems invs.
+
+Ltac pair_crush := pair_crush' False fail.
+
+Ltac reduce_preds :=
+  repeat match goal with
+    | |- appcontext[(_ && _)] => split; simpl
+    | [ H: appcontext[(_ && _)] |- _ ] => destruct H
+    | [ H: !!(_ = _) _ |- _ ] => destruct H (* This one is safe...? *)
+  end.
+
+Ltac crush_sep lems inv := 
+  crush' lems inv; reduce_preds;
+  repeat match goal with
+    | [ H : appcontext[(_ || _)] |- _ ] => destruct H
+    | [ H : (EX _ : _, _) _ |- _ ] => destruct H
+    | [ H : (_ && _) _ |- _ ] => destruct H; crush_sep lems inv
+    | [ H : _ (_ && _) _ |- _ ] => destruct H; crush_sep lems inv
+    | [ H : (_ |-- _), a : _ |- _ ] => specialize (H a); destruct H
+    | [ b : _, x : _ |- (EX _ : _, _) _ ] => exists (val_of_base b x)
+    | [ v : _  |- (EX _ : _, _) _ ] => exists v 
+    | [ v : nat |- (EX _ : value, _) _] => exists (int_v v)                                              
+    | [ v : bool |- (EX _ : value, _) _] => exists (bool_v v)                                              
+    | _ => idtac
+  end; crush.
+
+
+
+Ltac wf_expr H :=
+  let G := fresh "G" in
+  let v := fresh "v" in
+  let t := fresh "t" in
+  let NEQ := fresh "NEQ" in
+  let NotIn := fresh "NotIn" in
+  inversion H as
+      [ G v | G v t NEQ NotIn | G ].
+
+Ltac wf_prop H :=
+  let G := fresh "G" in
+  let b := fresh "b" in
+  let p := fresh "p" in
+  let p' := fresh "p'" in
+  let e1 := fresh "e1" in
+  let o := fresh "o" in
+  let e2 := fresh "e2" in
+  let WF:= fresh "WF" in
+  let WF':= fresh "WF'" in
+  inversion H as
+      [ G
+      | G e1 o e2 WF WF'
+      | G p WF
+      | G p p' WF WF'
+      | G p p' WF WF' ];
+    first [ wf_expr WF; wf_expr WF' | idtac].
+
+Ltac wf_ty H :=
+  let G := fresh "G" in
+  let b := fresh "b" in
+  let p := fresh "p" in
+  let WF:= fresh "WF" in
+      inversion H as [ G b p WF ]; wf_prop WF.
+                                                                             
+Ltac wellformed H :=
+  first [ wf_ty H | wf_prop H | wf_expr H ]; subst.
+
+(* Hint Rewrite subst_not_2. *)
+(* Hint Rewrite subst_not_1. *)
+
+Ltac app_pred := 
+  match goal with
+    | [ H: _ |- appcontext[sep_pred ?p] ] => 
+      match type of H with
+        | forall _:_, _ => fail 1
+        | _ -> _ => fail 1
+        | appcontext[sep_pred ?p] => (apply H || (intro; apply H) || (intros; apply H))
+      end
+  end.
+  
+Ltac commit t1 t2 t3 :=
+  (left; t1; t3) 
+  || (right; t2; t3).
+
+Ltac wf_crush :=
+  crush;
+  (do 2 match goal with 
+         | [ H: wf_prop _ ( _ _ _ ) |- _ ] => inversion H; subst
+         | [ H: wf_type _ { _ : _ | _ _ _ } |- _ ] => inversion H; subst
+         | [ H: wf_prop _ ( _ _ ) |- _ ] => inversion H; subst
+         | [ H: wf_type _ {_ : _ | _ _ } |- _ ] => inversion H; subst
+       end);
+  crush_sep False fail;
+  try app_pred.
+
+Ltac btapply k :=
+  match goal with
+    | [ H : appcontext[?f] |- ?f ] => destruct H; k
+    | [ H : forall _:?t, _, x:?t |- _ ] => specialize (H x); btapply k
+  end.
