TranslationLemmas.v
@@ -1,0 +1,114 @@
+Add LoadPath "vst".
+Require Import msl.msl_direct.
+Require Import Coq.Unicode.Utf8.
+
+Require Import Types.
+Require Import Judge.
+Require Import Translation.
+Require Import Language.
+Require Import ProgramLogic.
+Require Import WFLemmas.
+Require Import SubstLemmas.
+Require Import EvalLemmas.
+Require Import Tactics.
+
+Lemma type_interp :
+  forall Γ x T s,
+      sep_env Γ s -> (expr_type Γ (var_e x) T) -> sep_ty x T s.
+Proof.
+  intros Γ x [ ν b φ ] w SE ET.
+  unfold sep_ty.
+  inversion ET. subst.
+  split.
+  + unfold sep_base.
+    apply expr_eval_ty with (Γ := Γ) (φ := φ).
+    assumption. assumption.
+  + generalize dependent Γ. 
+    induction Γ. 
+    - intros. inversion H2.
+    - intros. apply in_inv in H2. destruct a. destruct H2.
+      * inversion H. subst. apply SE.
+      * apply IHΓ. unfold sep_env in SE.
+        {
+          apply SE. 
+        } 
+        {
+          apply H. 
+        } 
+        { 
+          inversion ET. 
+          subst.
+          apply in_inv in H3. destruct H3. 
+          { 
+            inversion H0. subst. constructor. apply H.
+          }
+          {
+            constructor. apply H0.
+          }
+        }
+Qed.
+
+Lemma sep_proof_skip :
+  forall Φ Γ Γ' (J : (Φ / Γ ⊢ skip_s ::: Γ')), 
+    {{ sep_env Γ }} skip_s {{ sep_env Γ' }}.
+Proof.
+  intros. inversion J. constructor.
+Qed.
+
+Lemma sep_proof_assign :
+  forall Φ Γ Γ' x e (J : (Φ / Γ ⊢ assign_s x e ::: Γ')), x <> ν -> 
+    {{ sep_env Γ }} assign_s x e {{ sep_env Γ' }}.
+Proof.
+  intros Φ Γ Γ' x e J NotVV.
+  inversion J. subst.
+  apply semax_pre_post with (P' := EX v : value, eval_to e v 
+                                              && subst_pred x e (sep_env ((x, {ν : τ | (var_e ν) .= e }) :: Γ)))
+                            (Q' := sep_env ((x,{ν : τ | (var_e ν) .= e }) :: Γ)).
+  unfold derives.
+  simpl.
+  intro w. intro SE.
+  assert (exists b, eval_to e b w) as ExVal.
+    apply expr_eval with (Γ := Γ) (T := { ν : τ | φ }). apply SE. apply H5.
+  destruct ExVal. exists x0.
+  split. apply H. simpl.
+  split. split.
+  inversion H5. 
+  unfold sep_base. subst. destruct v. simpl. exists n. destruct (eq_dec x x). reflexivity. contradiction n0. reflexivity.
+  exists b. simpl. destruct (eq_dec x x). reflexivity. contradiction n. reflexivity.
+  subst. unfold sep_base. 
+  apply expr_eval_ty with (Γ := Γ) (φ := φ). 
+
+exists x0.
+  apply subst_none_base with (x := x) (e := e).
+  destruct ExVal.
+  exists x0. 
+  split.
+    assumption. 
+    split. split. 
+    unfold sep_base. 
+    pose (expr_eval' Γ (var_e x) τ φ) as E'. 
+    eapply E'. 
+    split.
+    unfold derives in E'.
+    exists (val_of_base τ x0).
+        (* destruct H3. unfold imp in H1. apply H1. *)
+  split. split.
+    apply SE.
+    apply H5.
+  elim ExVal.
+    intro val. intro EvalTo.
+  exists val.
+  destruct t as [ν τ φ].
+  hnf.
+  split.
+    apply EvalTo.
+    split. split.
+
+(* (*** The main thingie ***) *)
+(* Theorem sep_type : *)
+(*   forall Φ Γ s Γ', *)
+(*     Φ / Γ ⊢ s ::: Γ' ->  *)
+(*     {{ sep_env Γ }} s {{ sep_env Γ' }}. *)
+(* Proof. *)
+(*   intros. *)
+(*   destruct s. *)
