WFLemmas.v
@@ -1,0 +1,85 @@
+Add LoadPath "vst".
+Require Import msl.msl_direct.
+Require Import Coq.Unicode.Utf8.
+
+Require Import Translation.
+Require Import Types.
+Require Import Judge.
+Require Import Language.
+Require Import Subst.
+Require Import Tactics.
+
+Lemma fresh_var :
+  forall x t Γ,
+    var_not_in x Γ -> In (x,t) Γ -> False.
+Proof.
+  unfold var_not_in in *; pair_crush.
+Qed.
+
+Lemma var_not_in_exp :
+  forall x e Γ,
+    (x <> ν) -> var_not_in x Γ -> wf_expr Γ e -> (e <> (var_e x)).
+Proof.
+  intros x e Γ neq not_in wf_exp;
+  inversion wf_exp; crush' fresh_var fail.
+Qed.
+
+Ltac wf_freshvar exp :=
+  match goal with
+    | [ x:var, G:type_env, V:var_not_in ?x ?G, H: wf_expr ?G _ |- _ ] => 
+      let V1 := fresh "V"  in
+      set (V1 := V);
+      eapply var_not_in_exp with (e := exp) in V1
+   end.
+
+Lemma wf_env_ty :
+  forall Γ x t, 
+    wf_env Γ -> (x, t) ∈ Γ -> wf_type Γ t.
+Proof.
+  pair_crush' False wf_env.
+Qed.
+
+Lemma wf_type_prop : 
+  forall Γ ν τ φ,
+    wf_type Γ { ν : τ | φ } -> wf_prop Γ φ.
+Proof.
+  pair_crush' False wf_type.
+Qed.
+
+Lemma wf_expr_subst :
+  forall Γ e x,
+    wf_expr Γ e -> var_in x Γ ->
+    wf_expr Γ (subst ((ν, x) :: nil) e).
+Proof.
+  intros; unfold var_in in *; destruct e; 
+  repeat
+    (match goal with
+       | [ |- context[subst _ _] ] => unfold subst; simpl
+       | [ |- context[eq_dec ?x ?v] ] => destruct (eq_dec x v)
+     end; crush' wf_var fail).
+Qed.
+
+Lemma wf_prop_subst :
+  forall Γ φ x,
+    wf_prop Γ φ -> var_in x Γ ->
+    wf_prop Γ (subst ((ν, x) :: nil) φ).
+Proof.
+  induction φ; intros; constructor; crush' wf_expr_subst ((wf_type, wf_prop), wf_expr).
+Qed.
+
+Lemma wf_env_prop :
+  forall Γ x ν τ φ, 
+    wf_env Γ -> (x, { ν : τ | φ }) ∈ Γ -> wf_prop Γ φ.
+Proof.
+  intros;
+  apply wf_type_prop with (ν := ν) (τ := τ);
+  apply wf_env_ty with (x := x); crush.
+Qed.
+
+Lemma wf_not_in :
+  forall x t x' Γ,
+    var_not_in x' Γ -> wf_type Γ t -> (x,t) ∈ Γ ->
+    x <> x'.
+Proof.
+  intros; unfold var_not_in in *; crush; app_pair; crush.
+Qed.
